added a dataflow network rocq thing

src/Dataflow.v
@@ -1,63 +1,100 @@
-From Stdlib Require Import Lists.List.
-From Stdlib Require Import Lists.ListSet.
-From DatalogRocq Require Import ComputeCore.
+From Stdlib Require Import List Bool.
 From Datalog Require Import Datalog.
+From coqutil Require Import Map.Interface Map.Properties Map.Solver Tactics Tactics.fwd Datatypes.List.
 
 Import ListNotations.
 
-(* Adjacency List Concrete Representation, plan to generalize later probably? *)
-Definition dataflow_graph := list (core_id * core_set).
+Section DistributedDatalog.
 
-Definition valid_graph (g: dataflow_graph) : Prop :=
-  NoDup (map fst g).
+  Context {rel var fn aggregator T : Type}.
+  Context `{sig : signature fn aggregator T}.
+  Context `{query_sig : query_signature rel}.
+  Context {context : map.map var T}.
+  Context {context_ok : map.ok context}.
+  Context {Node Info : Type}.
+  Context {node_eqb : Node -> Node -> bool}.
+  Context {node_eqb_spec : forall x y, BoolSpec (x = y) (x <> y) (node_eqb x y)}.
 
-Fixpoint get_outgoing_edges (g: dataflow_graph) (c: core_id) : core_set :=
-  match g with
-  | [] => empty_core_set
-  | (c', edges)::g' => if c =c c' then edges else get_outgoing_edges g' c
-  end.
+  Definition fact := Datalog.fact rel var fn.
+  Definition rule := Datalog.rule rel var fn aggregator.
 
-Fixpoint get_incoming_edges (g: dataflow_graph) (c: core_id) : core_set :=
-  match g with
-  | [] => empty_core_set
-  | (c', edges)::g' => let inc_edges := get_incoming_edges g' c in
-                if core_set_mem c edges then
-                  core_set_add c' inc_edges
-                else inc_edges
-  end.
-
-Definition get_cores (g: dataflow_graph) : core_set :=
-  fold_right (fun (ce: core_id * core_set) acc =>
-                let (c', edges) := ce in
-                core_set_add c' acc)
-             empty_core_set g.
-
-Definition has_edge (g: dataflow_graph) (c1 c2: core_id) : bool :=
-  core_set_mem c2 (get_outgoing_edges g c1).
-
-Definition reachable (g: dataflow_graph) (c1 c2: core_id) : Prop :=
-  exists path, path <> [] /\
-               hd_error path = Some c1 /\
-               last path c1 = c2 /\
-               (forall i, i + 1 < length path -> has_edge g (nth i path c1) (nth (i + 1) path c1) = true).
-
-Definition is_strongly_connected (g: dataflow_graph) : Prop :=
-  forall c1 c2, In c1 (get_cores g) -> In c2 (get_cores g) -> reachable g c1 c2.
-
-Definition latency := nat.
-
-(* Latency should be defined for all cores reachable by each other in the dataflow graph *)
-Definition latency_fn := core_id -> core_id -> option latency.
-
-Definition valid_latency (g: dataflow_graph) (lat: latency_fn) : Prop :=
-  forall c1 c2, reachable g c1 c2 -> exists l, lat c1 c2 = Some l.
-
-Record dataflow_network := 
-  {
-    df_graph: dataflow_graph;
-    df_latency: latency_fn
+  Record Graph := {
+    nodes : Node -> Prop;
+    edge : Node -> Node -> Prop
   }.
 
-Definition get_latency (network: dataflow_network) (c1 c2: core_id) : option latency :=
-  network.(df_latency) c1 c2.
+  Definition good_graph (g : Graph) := 
+   forall n1 n2, edge g n1 n2 -> nodes g n1 /\ nodes g n2.
 
+  Inductive path (g : Graph) : Node -> Node -> Prop :=
+    | path_nil n :
+        g.(nodes) n ->
+        path g n n 
+    | path_cons n1 n2 n3 :
+        g.(edge) n1 n2 ->
+        path g n2 n3 ->
+        path g n1 n3.
+  
+  Definition strongly_connected (g : Graph) : Prop :=
+    forall n1 n2, g.(nodes) n1 -> g.(nodes) n2 -> path g n1 n2.
+
+  Definition ForwardingFn := Node -> rel * list T -> option Node.
+  Definition Layout := Node -> list rule.
+
+  Record DataflowNetwork := {
+    graph : Graph;
+    forward : ForwardingFn;
+    layout : Layout
+  }.
+
+(* Is there a nicer way to represent this? Seems a bit handwavy or whatever...*)
+
+Inductive network_pftree (net : DataflowNetwork) : Node -> rel * list T -> Prop :=
+  | RuleApp n f r hyps :
+      In r (net.(layout) n) ->
+      Forall (network_pftree net n) hyps ->
+      Datalog.rule_impl r f hyps ->
+      network_pftree net n f
+  | Forward n n' f :
+      network_pftree net n f ->
+      net.(forward) n f = Some n' ->
+      network_pftree net n' f.
+
+Definition network_prog_impl_fact (net : DataflowNetwork) : rel * list T -> Prop :=
+  fun f => exists n, network_pftree net n f.
+    
+Definition rule_assigned_to_node (layout : Layout) (r : rule) (n : Node) : Prop :=
+  In r (layout n).
+
+(* A good layout has every program rule on a node somewhere AND only assigns rules from 
+   the program to nodes*)
+Definition good_layout (layout : Layout) (nodes : Node -> Prop) (program : list rule) : Prop :=
+   Forall (fun r => exists n, nodes n /\ rule_assigned_to_node layout r n) program /\
+   forall n r, nodes n /\ rule_assigned_to_node layout r n -> In r program.
+
+(* A good forwarding function should only be able to forward things along the 
+   edges *)
+Definition good_forwarding (forward : ForwardingFn) (nodes : Node -> Prop) (edges : Node -> Node -> Prop) : Prop :=
+  forall n1 n2 f, forward n1 f = Some n2 -> nodes n1 /\ nodes n2 /\ edges n1 n2.  
+
+Definition good_network (net : DataflowNetwork) (program : list rule) : Prop :=
+  good_graph net.(graph) /\
+  good_layout net.(layout) net.(graph).(nodes) program /\
+  good_forwarding net.(forward) net.(graph).(nodes) net.(graph).(edge).
+
+
+(* These aren't necessarily true in general, we have to consider our layout and 
+   forwarding function to make this true, but these are placeholders for now for the 
+   possible coming definitions. *)
+
+Theorem soundness (net : DataflowNetwork) (program : list rule) :
+  forall f, network_prog_impl_fact net f -> Datalog.prog_impl_fact program f.
+Admitted.
+
+Theorem completeness (net : DataflowNetwork) (program : list rule) :
+  forall f, Datalog.prog_impl_fact program f -> 
+  good_network net program ->
+  network_prog_impl_fact net f.
+Admitted.
+
+End DistributedDatalog.
